prover integration into symbolic evaluation. - things have gotten very slow!

examples/AutoSep.v
@@ -4,29 +4,72 @@ Export Bedrock.
 (** * Specialize the library proof automation to some parameters useful for basic examples. *)
 
 Import SymIL.BedrockEvaluator.
-Require Import Bedrock.sep.PtsTo2.
+Require Bedrock.sep.PtsTo2.
+
+(** Build our memory plugin **)
+Module Plugin_PtsTo := Bedrock.sep.PtsTo2.BedrockPtsToEvaluator SymIL.PLUGIN.
+
+Definition master_plugin types' :=
+  let types := Env.repr SymIL.bedrock_types_r types' in
+  @PluginEvaluator.Plugin_SymEvaluator types (Expr.tvType 0) (Expr.tvType 1)
+  ((0, Plugin_PtsTo.MemEval_ptsto32 _) :: nil).
+
+Definition master_plugin_correct types' (_ _ : Expr.tvar) funcs sfuncs : 
+  (forall F, F sfuncs -> F (Plugin_PtsTo.ptsto32_ssig _ :: tl sfuncs)) ->
+  SymEvaluator_correct funcs sfuncs (master_plugin types').
+Proof.
+  simpl in *. intros.
+  generalize PluginEvaluator.Plugin_SymEvaluator_correct.
+  unfold master_plugin, PluginEvaluator.pcT, PluginEvaluator.stT.
+Admitted.
+
+Ltac prover_unfolder H :=
+  match H with
+    | tt => 
+      cbv delta [
+        EquivDec_nat
+        Provers.transitivityProver
+        Provers.transitivity_summary Provers.transitivitySummarize Provers.transitivityLearn Provers.transitivityProve
+        Provers.transitivityEqProver
+        Provers.in_seq Provers.inSameGroup Provers.eqD_seq
+        Provers.groupsOf Provers.groupWith Provers.addEquality
+      ]
+    | _ => 
+      cbv delta [
+        EquivDec_nat
+        Provers.transitivityProver
+        Provers.transitivity_summary Provers.transitivitySummarize Provers.transitivityLearn Provers.transitivityProve
+        Provers.transitivityEqProver
+        Provers.in_seq Provers.inSameGroup Provers.eqD_seq
+        Provers.groupsOf Provers.groupWith Provers.addEquality
+      ] in H
+  end.
 
 Ltac unfolder H :=
+  prover_unfolder H ;
   cbv delta [
-    ptsto_evaluator CORRECTNESS READER WRITER DEMO.expr_equal DEMO.types
-    DEMO.ptsto32_ssig DEMO.ptrIndex DEMO.wordIndex
-    SymEval.fold_args SymEval.fold_args_update
+    master_plugin PluginEvaluator.Plugin_SymEvaluator
+    Plugin_PtsTo.MemEval_ptsto32
+    Plugin_PtsTo.sym_read_word_ptsto32
+    Plugin_PtsTo.sym_write_word_ptsto32
+    Plugin_PtsTo.expr_equal
   ] in H;
-  sym_evaluator H.
+  PluginEvaluator.unfolder H.
 
 Ltac the_cancel_simplifier :=
+  prover_unfolder tt ;
   cbv beta iota zeta delta 
     [ SepTac.SEP.CancelSep projT1
       SepTac.SEP.hash SepTac.SEP.hash' SepTac.SEP.sepCancel
 
       SepExpr.FM.fold
 
-      Provers.eq_summary Provers.eq_summarize Provers.eq_prove 
-      Provers.transitivityEqProverRec
+      Provers.Learn Provers.Summarize Provers.Prove 
+      Provers.transitivityProver
 
       ExprUnify.Subst
 
-      SymIL.bedrock_types SymIL.bedrock_ext
+      SymIL.bedrock_types_r SymIL.bedrock_types
       app map fold_right nth_error value error
 
       fst snd
@@ -44,7 +87,7 @@ Ltac the_cancel_simplifier :=
       SepTac.SEP.unify_remove_all SepTac.SEP.unify_remove
 
       SepTac.SEP.unifyArgs
-      ExprUnify.fold_left_2_opt
+      ExprUnify.fold_left_2_opt ExprUnify.fold_left_3_opt
       Compare_dec.lt_eq_lt_dec nat_rec nat_rect 
 
       ExprUnify.exprUnify SepTac.SEP.substV length ExprUnify.Subst_lookup ExprUnify.Subst_replace
@@ -57,16 +100,12 @@ Ltac the_cancel_simplifier :=
       ExprUnify.get_Eq
       Expr.Eq
       EquivDec.nat_eq_eqdec
-      Provers.inSameGroup Provers.eqD_seq Provers.transitivityEqProver
 
-      Provers.groupsOf
-      Provers.addEquality
-      Provers.in_seq_dec
+(*      Provers.in_seq_dec *)
       Expr.typeof 
       Expr.expr_seq_dec
       Expr.tvarD
       Expr.tvar_val_sdec 
-      Provers.groupWith
       Expr.Range Expr.Domain Expr.Denotation
       Expr.well_typed 
       Expr.all2
@@ -74,20 +113,33 @@ Ltac the_cancel_simplifier :=
       SepTac.SEP.forallEach
       SepTac.SEP.sheapD SepTac.SEP.sexprD
       SepTac.SEP.starred SepTac.SEP.himp
-      Expr.Impl
+      Expr.Impl Expr.Impl_
 
       Expr.is_well_typed Expr.exprD Expr.applyD
 
       tvWord
+
+      orb
+      SymIL.BedrockEvaluator.pcT SymIL.BedrockEvaluator.stT
     ].
 
 Ltac vcgen :=
   structured_auto; autorewrite with sepFormula in *; simpl in *;
     unfold starB, hvarB, hpropB in *; fold hprop in *.
 
-Ltac evaluate := sym_eval ltac:isConst idtac unfolder (CORRECTNESS ptsto_evaluator) tt tt tt.
+Ltac evaluate := 
+  let plg ts pcT stT fs ps :=
+    constr:(@master_plugin_correct ts pcT stT fs ps (fun _ x => x))
+  in
+  let prv ts fs :=
+    constr:(@Provers.transitivityProver_correct ts fs)
+  in
+  sym_eval ltac:isConst prv plg idtac unfolder.
 
-Ltac cancel := sep_canceler ltac:(isConst) (@Provers.transitivityEqProverRec) the_cancel_simplifier tt.
+Ltac cancel :=
+  sep_canceler ltac:(isConst) 
+    ltac:(fun ts fs => constr:(@Provers.transitivityProver_correct ts fs))
+    the_cancel_simplifier tt.
 
 Ltac unf := unfold substH.
 Ltac reduce := Programming.reduce unf.
